ulib/LowStar.Permissions.fst
@@ -2,27 +2,27 @@ module LowStar.Permissions
 
 module F = FStar.FunctionalExtensionality
 
-open FStar.Real 
+open FStar.Real
 
 
 type permission = r:real{r >=. 0.0R /\ r <=. 1.0R}
 
-type perm_id = pos
+abstract type perm_id : eqtype = pos
 
-let allows_read (p:permission) : GTot bool =  
+let allows_read (p:permission) : GTot bool =
   p >. 0.0R
 
 let allows_write (p: permission) : GTot bool =
   p = 1.0R
 
 
-noeq type perms_rec (a: Type0) = {
+abstract noeq type perms_rec (a: Type0) = {
   current_max : perm_id;
   owner: perm_id;
   perm_map    : F.restricted_t perm_id (fun (x:perm_id) -> permission & a)
 }
 
-let get_permission_from_pid (#a: Type0) (p: perms_rec a) (pid: perm_id) : GTot permission =
+abstract let get_permission_from_pid (#a: Type0) (p: perms_rec a) (pid: perm_id) : GTot permission =
   let (perm, _) = p.perm_map pid in
   perm
 
@@ -32,61 +32,64 @@ let is_live_pid (#a: Type0) (v_perms: perms_rec a) (pid:perm_id) : GTot bool =
 
 type live_pid (#a: Type0) (v_perms: perms_rec a) = pid:perm_id{is_live_pid v_perms pid}
 
-let get_snapshot_from_pid (#a: Type0) (p: perms_rec a) (pid: perm_id) : GTot a =
+abstract let get_snapshot_from_pid (#a: Type0) (p: perms_rec a) (pid: perm_id) : GTot a =
   let (_, snap) = p.perm_map pid in snap
 
+abstract let is_pid_owner (#a: Type0) (p: perms_rec a) (pid: perm_id) : GTot bool =
+  pid = p.owner
 
-
-let rec sum_until (#a: Type0) (f:perm_id -> permission & a) (n:nat) : GTot real =
+private let rec sum_until (#a: Type0) (f:perm_id -> permission & a) (n:nat) : GTot real =
   if n = 0 then 0.0R
-  else 
+  else
     let (x, _) = f n in x +. sum_until f (n - 1)
 
 let value_perms (a: Type0) = p:perms_rec a{
   // Permissions are null above currently split objects
   (forall (n:perm_id). n > p.current_max ==> get_permission_from_pid p n = 0.R) /\
   // The sum of permissions is the number of splits up till now
-  (sum_until p.perm_map p.current_max = 1.0R) /\ 
+  (sum_until p.perm_map p.current_max = 1.0R) /\
   // All permissions have the same snapshot
   (forall (pid1 pid2: perm_id). let snap1 = get_snapshot_from_pid p pid1 in let snap2 = get_snapshot_from_pid p pid2 in
      snap1 == snap2
   )
 }
 
-let new_value_perms (#a: Type0) (init: a) : Ghost (value_perms a)
-  (requires (True)) (ensures (fun v_perms -> 
+abstract let new_value_perms (#a: Type0) (init: a) : Ghost (value_perms a & perm_id)
+  (requires (True)) (ensures (fun (v_perms, pid) ->
+    get_permission_from_pid v_perms pid = 1.0R /\
+    is_pid_owner v_perms pid /\
     (forall (pid:perm_id).{:pattern get_snapshot_from_pid v_perms pid}
       get_snapshot_from_pid v_perms pid == init
     )
   ))
   =
-  let f:F.restricted_t perm_id (fun (x:perm_id) -> permission & a) = 
-     F.on_dom perm_id (fun (x:perm_id) -> if x = 1 then 
-         ((1.0R <: permission), init) 
-       else 
+  let f:F.restricted_t perm_id (fun (x:perm_id) -> permission & a) =
+     F.on_dom perm_id (fun (x:perm_id) -> if x = 1 then
+         ((1.0R <: permission), init)
+       else
          ((0.0R <: permission), init)
-     )   
+     )
   in
-  { current_max = 1; perm_map = f; owner = 1 }
+  ({ current_max = 1; perm_map = f; owner = 1 }, 1)
 
 type permission_kind =
-  | DEAD 
+  | DEAD
   | RO
   | RW
   | FULL
 
-let get_perm_kind_from_pid (#a: Type0) (perms: value_perms a) (pid: perm_id) : GTot permission_kind = 
+let get_perm_kind_from_pid (#a: Type0) (perms: value_perms a) (pid: perm_id) : GTot permission_kind =
   let permission = get_permission_from_pid perms pid in
   if permission = 0.0R then
     DEAD
-  else if permission <. 1.0R then 
+  else if permission <. 1.0R then
     RO
-  else if perms.owner <> pid then
+  else if is_pid_owner perms pid  then
     RW
-  else 
+  else
     FULL
 
-let rec same_prefix_same_sum_until(#a: Type0) (p1 p2:perm_id -> permission & a) (n:nat) : Lemma
+private let rec same_prefix_same_sum_until(#a: Type0) (p1 p2:perm_id -> permission & a) (n:nat) : Lemma
   (requires forall (x:perm_id). x <= n ==> begin
     let (perm1, _) = p1 x in let (perm2, _) = p2 x in
     perm1 = perm2
@@ -94,33 +97,33 @@ let rec same_prefix_same_sum_until(#a: Type0) (p1 p2:perm_id -> permission & a) 
   (ensures sum_until p1 n = sum_until p2 n)
   = if n = 0 then () else same_prefix_same_sum_until p1 p2 (n-1)
 
-let rec sum_until_change 
-  (#a: Type0) 
+private let rec sum_until_change
+  (#a: Type0)
   (p1 p2:perm_id -> permission & a)
   (n:nat)
   (i:perm_id)
-  (v:permission) 
-  : Lemma (requires (forall (x:perm_id). 
+  (v:permission)
+  : Lemma (requires (forall (x:perm_id).
     let (v1, _) = p1 x in let (v2, _) = p2 x in
     (x <= n /\ x <> i) ==> v1 = v2) /\
     i <= n /\
     begin let (v', _) = p2 i in v' = v end
   ) (ensures (let (v', _) = p1 i in sum_until p2 n = sum_until p1 n +. v -. v'))
-  = 
+  =
     if n = i then same_prefix_same_sum_until p1 p2 (n-1)
     else sum_until_change p1 p2 (n-1) i v
 
-let share_perms (#a: Type0) (v_perms: value_perms a) (pid: live_pid v_perms) : Ghost (value_perms a & perm_id)  
-  (requires (True)) (ensures (fun (new_v_perms, new_pid) -> 
+abstract let share_perms (#a: Type0) (v_perms: value_perms a) (pid: live_pid v_perms) : Ghost (value_perms a & perm_id)
+  (requires (True)) (ensures (fun (new_v_perms, new_pid) ->
     new_pid <> pid /\
     get_permission_from_pid new_v_perms pid = get_permission_from_pid v_perms pid /. 2.0R /\
     get_permission_from_pid new_v_perms new_pid = get_permission_from_pid v_perms pid /. 2.0R /\
-    (forall (pid':perm_id{pid' <> pid /\ pid' <> new_pid}).{:pattern get_permission_from_pid new_v_perms pid'} 
+    (forall (pid':perm_id{pid' <> pid /\ pid' <> new_pid}).{:pattern get_permission_from_pid new_v_perms pid'}
       get_permission_from_pid v_perms pid' == get_permission_from_pid new_v_perms pid'
     ) /\
     (forall (pid':perm_id).{:pattern get_snapshot_from_pid new_v_perms pid'}
       get_snapshot_from_pid v_perms pid' == get_snapshot_from_pid new_v_perms pid'
-    )    
+    )
   ))
   =
   let current_max' = v_perms.current_max + 1 in
@@ -136,22 +139,22 @@ let share_perms (#a: Type0) (v_perms: value_perms a) (pid: live_pid v_perms) : G
   in
   sum_until_change perm_map1' perm_map2' current_max' current_max' (p /. 2.0R);
   let v_perms' : perms_rec a =
-    { v_perms with 
-      current_max = current_max'; 
+    { v_perms with
+      current_max = current_max';
       perm_map = perm_map2'
     }
   in
   (v_perms', current_max')
 
 
-let rec sum_greater_than_subterm (#a: Type0) (f:perm_id -> permission & a) (n:nat) (pid1:perm_id)
+private let rec sum_greater_than_subterm (#a: Type0) (f:perm_id -> permission & a) (n:nat) (pid1:perm_id)
   : Lemma (ensures (
     if n < pid1 then sum_until f n >=. 0.0R else
     sum_until f n >=. (let (x, _) = f pid1 in x)
   )) =
   if n = 0 then () else sum_greater_than_subterm f (n-1) pid1
 
-let rec sum_greater_than_subterms (#a: Type0) (f:perm_id -> permission & a) (n:nat) (pid1: perm_id)
+private let rec sum_greater_than_subterms (#a: Type0) (f:perm_id -> permission & a) (n:nat) (pid1: perm_id)
   (pid2:perm_id{pid1 <> pid2})
   : Lemma (ensures (
     let (pid1, pid2) = if pid1 < pid2 then (pid1, pid2) else (pid2, pid1) in
@@ -161,15 +164,15 @@ let rec sum_greater_than_subterms (#a: Type0) (f:perm_id -> permission & a) (n:n
   )) =
   if n = 0 then () else sum_greater_than_subterms f (n-1) pid1 pid2
 
-let merge_perms
+abstract let merge_perms
   (#a: Type0)
   (v_perms: value_perms a)
   (pid1: live_pid v_perms)
-  (pid2: live_pid v_perms{pid1 <> pid2}) 
-  : Ghost (value_perms a & perm_id) 
-  (requires (True)) (ensures (fun (new_v_perms, new_pid) -> 
+  (pid2: live_pid v_perms{pid1 <> pid2})
+  : Ghost (value_perms a & perm_id)
+  (requires (True)) (ensures (fun (new_v_perms, new_pid) ->
     new_pid = pid1 /\
-    get_permission_from_pid new_v_perms new_pid = 
+    get_permission_from_pid new_v_perms new_pid =
       get_permission_from_pid v_perms pid1 +. get_permission_from_pid v_perms pid2 /\
     get_permission_from_pid new_v_perms pid2 = 0.0R /\
     (forall (pid':perm_id{pid' <> pid1 /\ pid' <> pid2}).{:pattern get_permission_from_pid new_v_perms pid'}
@@ -179,7 +182,7 @@ let merge_perms
       get_snapshot_from_pid v_perms pid' == get_snapshot_from_pid new_v_perms pid'
     )
   ))
-  = 
+  =
   let (p1, snap1) = v_perms.perm_map pid1 in
   let (p2, snap2) = v_perms.perm_map pid2 in
   sum_greater_than_subterms v_perms.perm_map v_perms.current_max pid1 pid2;
@@ -190,7 +193,7 @@ let merge_perms
     else v_perms.perm_map x
   ) in
   sum_until_change v_perms.perm_map perm_map1' v_perms.current_max pid1 p_sum;
-  let perm_map2' = F.on_dom perm_id (fun (x:perm_id) -> 
+  let perm_map2' = F.on_dom perm_id (fun (x:perm_id) ->
     if x = pid2 then ((0.0R <: permission), snap2) else perm_map1' x
   ) in
   sum_until_change perm_map1' perm_map2' v_perms.current_max pid2 0.0R;
@@ -198,9 +201,9 @@ let merge_perms
     {  v_perms with perm_map = perm_map2' } in
   (v_perms', pid1)
 
-let change_snapshot (#a: Type0) (v_perms: value_perms a) (new_snapshot: a) 
+abstract let change_snapshot (#a: Type0) (v_perms: value_perms a) (new_snapshot: a)
   : Ghost (value_perms a)
-  (requires (True)) (ensures (fun new_v_perms -> 
+  (requires (True)) (ensures (fun new_v_perms ->
     (forall (pid:perm_id).{:pattern get_permission_from_pid new_v_perms pid}
       get_permission_from_pid new_v_perms pid = get_permission_from_pid v_perms pid
     ) /\
@@ -209,11 +212,10 @@ let change_snapshot (#a: Type0) (v_perms: value_perms a) (new_snapshot: a)
     )
   ))
   =
-  let out = { v_perms with 
+  let out = { v_perms with
     perm_map = F.on_dom perm_id (fun (x:perm_id) ->
       let (p, _) = v_perms.perm_map x in (p, new_snapshot)
     )
   } in
   same_prefix_same_sum_until v_perms.perm_map out.perm_map v_perms.current_max;
   out
-
